src/Common/Notations.v
@@ -1,0 +1,4 @@
+Reserved Notation "# x" (at level 70).
+Reserved Infix "@" (left associativity, at level 77).
+Reserved Notation "\ x , e" (at level 78).
+Reserved Notation "\ ! , e" (at level 78).
