src/Parsers/Reflective/ParserSyntaxEquivalence.v
@@ -1,0 +1,22 @@
+(** * Equivalence on syntax *)
+Require Import Fiat.Parsers.Reflective.Syntax Fiat.Parsers.Reflective.ParserSyntax.
+Require Import Fiat.Parsers.Reflective.SyntaxEquivalence.
+
+Section has_parse_term_equiv.
+  Context (var1 var2 : TypeCode -> Type).
+
+  Inductive has_parse_term_equiv : ctxt var1 var2 -> has_parse_term var1 -> has_parse_term var2 -> Prop :=
+  | EqFix2
+      (G_length : nat) (up_to_G_length : list nat)
+      (valid_len : nat)
+      (valids : list nat)
+      (nt_idx : nat)
+    : forall G f1 f2,
+      Term_equiv G f1 f2
+      -> has_parse_term_equiv
+           G
+           (RFix2 G_length up_to_G_length f1 valid_len valids nt_idx)
+           (RFix2 G_length up_to_G_length f2 valid_len valids nt_idx)
+  | EqRefl' : forall (E : polyhas_parse_term),
+      has_parse_term_equiv nil (E var1) (E var2).
+End has_parse_term_equiv.
