src/Parsers/Reflective/SyntaxEquivalence.v
@@ -1,0 +1,41 @@
+(** * Equivalence on syntax *)
+Require Import Coq.Lists.List.
+Require Import Fiat.Parsers.Reflective.Syntax.
+
+Local Open Scope list_scope.
+
+Section Term_equiv.
+  Context (var1 var2 : TypeCode -> Type).
+
+  Definition vpair := { t : TypeCode & var1 t * var2 t }%type.
+  Definition vars t (x1 : var1 t) (x2 : var2 t) : vpair := existT _ _ (x1, x2).
+  Definition ctxt := list vpair.
+
+  Inductive Term_equiv : ctxt -> forall {t}, Term var1 t -> Term var2 t -> Prop :=
+  | EqVar : forall G t (v1 : var1 t) v2,
+    List.In (vars v1 v2) G
+    -> Term_equiv G (#v1) (#v2)
+
+  | EqLiteralApp : forall G T f v1 v2,
+      args_for_equiv G v1 v2
+      -> Term_equiv G (@RLiteralApp var1 T f v1) (@RLiteralApp var2 T f v2)
+
+  | EqApp : forall G t1 t2 (f1 : Term _ (t1 --> t2)) (x1 : Term _ t1) f2 x2,
+    Term_equiv G f1 f2
+    -> Term_equiv G x1 x2
+    -> Term_equiv G (f1 @ x1) (f2 @ x2)
+  | EqLambda : forall G t1 t2 (f1 : var1 t1 -> Term var1 t2) f2,
+    (forall v1 v2, Term_equiv (vars v1 v2 :: G) (f1 v1) (f2 v2))
+    -> Term_equiv G (RLambda f1) (RLambda f2)
+  | EqRefl : forall T (E : polyTerm T),
+      Term_equiv nil (E var1) (E var2)
+  with args_for_equiv : ctxt -> forall {t}, args_for var1 t -> args_for var2 t -> Prop :=
+       | Eq_an_arg {G A B} (arg1 : Term var1 A) (arg2 : Term var2 A)
+                   (args1 : args_for var1 B) (args2 : args_for var2 B)
+         : Term_equiv G arg1 arg2
+           -> args_for_equiv G args1 args2
+           -> args_for_equiv G (an_arg arg1 args1) (an_arg arg2 args2)
+       | Eq_noargs {G T} : args_for_equiv G (@noargs var1 T) (@noargs var2 T).
+End Term_equiv.
+
+Arguments vars {var1 var2 t} _ _.
